\begin{problem}
    {Q1(a)}
    $4-SAT$: Each clause has exactly 4 variables. \\
    Prove or disprove: $4-SAT$ is NP-Complete \\
    \textbf{Claim}: $4-SAT$ is NP-Complete \\
    \textbf{Poly-time reduction}
    \begin{algorithmic}[1]
        \STATE Let $\Phi$ be an expression of a 3-SAT problem
        \STATE Let $\Phi'$ be an initially empty expression
        \FOR {$\forall C_j = (x \lor y \lor z) \in \Phi$ where $x,y,z$ are literals}
            \STATE Create a new boolean variable $\alpha$
            \STATE $C^1_j := (x \lor y \lor z \lor \alpha)$
            \STATE $C^2_j := (x \lor y \lor z \lor \overline{\alpha})$
            $\Phi' := \Phi \land C^1_j \land C^2_j$ \\
        \ENDFOR
        \RETURN {$4-SAT(\Phi')$}
    \end{algorithmic}
    \noindent
    \textbf{Proof of Correctness}
    \begin{proof}
        Take $(x \lor y \lor z \lor \alpha) \land (x \lor y \lor z \lor \overline{\alpha})$ \\
        $ = ( (x \lor y \lor z) \lor \alpha) \land ( (x \lor y \lor z) \lor
        \overline{\alpha})$ \\
        $ = ((x \lor y \lor z) \land (x \lor y \lor z)) \lor ((x \lor y \lor z) \land \overline{\alpha}) \lor (\alpha \land (x \lor y \lor z)) \lor
        (\alpha \land \overline{\alpha})$ \\
        $ = (x \lor y \lor z) \lor ((x \lor y \lor z) \land \overline{\alpha}) \lor (\alpha \land (x \lor y \lor z))$ \\
        $ = (x \lor y \lor z) \lor \left(((x \lor y \lor z) \land \overline{\alpha}) \lor (\alpha \land (x \lor y \lor z))\right)$ \\
        $ = (x \lor y \lor z) \lor \left((x \lor y \lor z) \land (\overline{\alpha} \lor \alpha)\right)$ \\
        $ = (x \lor y \lor z) \lor ((x \lor y \lor z) \land T)$ \\
        $ = (x \lor y \lor z) \lor (x \lor y \lor z)$ \\
        $ = (x \lor y \lor z)$ \\
        Therefore, $(x \lor y \lor z \lor \alpha) \land (x \lor y \lor z \lor \overline{\alpha}) = (x \lor y \lor z)$ \\
        By line 5-6, every clause $C_j \in \Phi$ is transformed into an equivalent set of two clauses $C^1_j, C^2_j \in \Phi'$ \\
        Now, by the associative property,
        $C^1_1 \land C^2_1 \land C^1_2 \land C^2_2 \dots \land C^1_n \land C^2_n$
        $ = (C^1_1 \land C^2_1) \land \dots \land (C^1_n \land C^2_n)$ \\
        By the previous proof, we have established $(C^1_j \land C^2_j) = C_j$ \\
        Therefore, $\Phi' = C_1 \land C_2 \land \dots \land C_n$ \\
        Therefore, $\Phi' = \Phi$ which means $4-SAT$ can solve any 3-SAT problem $\Phi$ by using the above reduction. \\
    \end{proof}
    \noindent
    \textbf{Proof of Runtime}
    \begin{proof}
        Let the number of clauses in $C_j$ be expressed as $N$
        The reduction processes each clause $C_j \in \Phi$ once and generates two new clauses $C^1_j, C^2_j$ \\
        Therefore, the runtime is $\theta(2N) = \theta(N)$ which is polynomial in $N$ \\
        Therefore, if the reduction is correct, $3-SAT \leq_{p} 4-SAT$ \\
    \end{proof}
\end{problem}
